coq-SystemRF-3.0/SystemRF/MainTheorems.v
@@ -8,6 +8,8 @@ Require Import SystemRF.WellFormedness.
 Require Import SystemRF.PrimitivesFTyping.
 Require Import SystemRF.BasicPropsWellFormedness.
 Require Import SystemRF.Typing.
+Require Import SystemRF.LemmasWeakenTyp.
+Require Import SystemRF.LemmasWellFormedness.
 Require Import SystemRF.LemmasTyping.
 Require Import SystemRF.LemmasSubtyping.
 Require Import SystemRF.LemmasExactness.
@@ -16,6 +18,9 @@ Require Import SystemRF.SubstitutionLemmaTypTV.
 Require Import SystemRF.LemmasNarrowing.
 Require Import SystemRF.LemmasInversion.
 Require Import SystemRF.PrimitivesDeltaTyping.
+
+Require Import Arith.
+Require Import ZArith.
 
 (*--------------------------------------------------------------------------------
 --- | PROGRESS and PRESERVATION  
@@ -201,7 +206,7 @@ Proof. intros g e t e' p_e_t; revert e'; induction p_e_t;
       destruct Hfv; destruct Hfr; try simpl in H3;
       try apply not_elem_union_elim in H3; try destruct H3;
       try apply WFEEmpty; intuition. 
-    * (* App (AppT Length t) *)
+    * (* App (AppT Length t) val *)
       destruct e0 eqn:E0; try contradiction;
       destruct p eqn:P; try contradiction.
       assert (isCompatM' Length e') as pf
@@ -213,56 +218,42 @@ Proof. intros g e t e' p_e_t; revert e'; induction p_e_t;
         by (apply TApp; assumption).
       apply lem_sem_det 
         with (App (AppT (Prim Length) t0) e') e'' (deltaM Length e' pf) 
-        in st_e_e'' as He''; try apply EPrimM; try assumption. 
-      subst e''; inversion pf; subst e';
+        in st_e_e'' as He''; try apply EPrimM; try assumption.
+      pose proof (lem_deltaM_typ Length t0 e' t_x t) as He'''.
+      destruct He''' as [e''' [He''' p_e''_txt]]; trivial.
+      rewrite <- deltaM_deltaM' with Length e' pf in He''';
+      injection He''' as He'''; subst e'' e'''; apply p_e''_txt.
 
-      inversion p_e_t2; subst t_x.
-      simpl.
-
-        pose proof lem_deltaM_typ.
-
-        pose proof lem_deltaM_ftyp.
-    | EPrimM : forall (c : prim) (t : type) (w : expr) (pf : isCompatM c w),
-          isValue w -> Step (App (AppT (Prim c) t) w) (deltaM c w pf) 
-
-        inversion H7; rewrite <- H19 in H6; unfold ftsubBV in H6; 
-        injection H6 as H6 H6'; subst b. 
-        
-        apply lem_deltaM_ftyp with Length k t' e2 (erase t) in H4 as He'; 
-        simpl; trivial.  destruct He' as [del He']; destruct He'.
-        assert (del = deltaM Length e2 pf)
-          by (rewrite <- (deltaM_deltaM' Length e2 pf) in H16; 
-              injection H16 as H16; assumption).
-        subst del; assert (e' = deltaM Length e2 pf)
-          by (apply lem_sem_det with (App (AppT (Prim Length) t) e2); 
-              try apply EPrimM; assumption);
-        subst e' t0 b'; assumption.
-  - (* TAppT e t *) apply thm_progress in p_e_t as Hprog;
-    destruct e eqn:E; simpl in Hprog;
-    (* impossible cases: *)
-    apply lem_typing_hasftype in p_e_t as p_e_ert; try simpl in p_e_ert;
-    try assert (isValue e) as Hval by (subst e; simpl; tauto); try apply WFEEmpty;
-    try apply lemma_tfunction_values with e k (erase s) in Hval as Hfval;
-    try (rewrite E; apply p_e_ert);
-    try (subst e; simpl in Hfval; contradiction);
+  - (* TAppT e t *) apply thm_progress in p_e_t as Hprog; 
+    destruct Hprog;
     (* e not value: *)
-    rewrite <- E in st_e_e'';
-    try assert (exists e1 : expr, Step e e1) as HStep1 
-        by (rewrite E; intuition; apply Hprog);
-    try ( destruct HStep1 as [e1 HStep1]; 
-          apply lem_sem_det with (AppT e t) e'' (AppT e1 t) in st_e_e'' as He'';
-          try apply EAppT; try assumption; subst e'';
-          apply TAppT with k; try apply IHp_e_t; subst e; trivial ).
+    try destruct H2 as [e' st_e_e'];
+    try apply lem_sem_det with (AppT e t) e'' (AppT e' t)
+      in st_e_e'' as He'';
+    try apply EAppT; try assumption; try subst e'';
+    try apply TAppT with k; try apply IHp_e_t; trivial.
+    (* e is a value *) 
+    apply lem_typing_hasftype in p_e_t as p_e_ert;
+    try simpl in p_e_ert; try apply WFEEmpty.    
+    apply lemma_tfunction_values in p_e_ert as Hfval; 
+    try apply H2; destruct e eqn:E; simpl in Hfval; try contradiction.
     * (* AppT (Prim p) t *) 
+      assert (isMeasure p \/ ~ isMeasure p) as nomeas
+        by (destruct p; intuition).
+      destruct nomeas as [meas|nomeas];
+      try ( destruct p; simpl in meas; try contradiction;
+            apply lem_value_stuck in st_e_e''; 
+            try apply val_Len; contradiction ). 
       assert (Hastype Empty (AppT (Prim p) t) (tsubBTV t s))
         by (apply TAppT with k; assumption).
-      pose proof (lem_prim_compatT_in_tappT p t (tsubBTV t s) H0 H2) as pf;
+      pose proof (lem_prim_compatT_in_tappT p t (tsubBTV t s) 
+                                            nomeas H0 H3) as pf;
       apply compatT_prop_set in pf; subst e;
       apply lem_sem_det with (AppT (Prim p) t) e'' (deltaT p t pf) in st_e_e'' 
         as He''; try apply EPrimT; try assumption; subst e'';
-      pose proof (lem_deltaT_typ p t k s H H0 p_e_t H1) as He'';
+      pose proof (lem_deltaT_typ p t k s nomeas H H0 p_e_t H1) as He'';
       rewrite deltaT_deltaT' with p t pf in He''; destruct He'';
-      destruct H3; injection H3 as H3; subst x; assumption.
+      destruct H4; injection H4 as H4; subst x; assumption.
     * (* App (Lambda e0) val *) subst e;
       assert (Hastype Empty (AppT (LambdaT k0 e0) t) (tsubBTV t s)) as p_et_st
         by (apply TAppT with k; assumption);
@@ -280,18 +271,18 @@ Proof. intros g e t e' p_e_t; revert e'; induction p_e_t;
       try rewrite lem_tsubFTV_unbind_tvT with a t s;
       try apply lem_subst_tv_typ_top with k0; try apply p_e0_s;
       pose proof lem_fv_bound_in_fenv FEmpty (LambdaT k0 e0) 
-                    (FTPoly k0 (erase s)) a p_e_ert as Hfv;  
+                    (FTPoly k0 (erase s)) a p_e_ert as Hfv;
       pose proof lem_free_bound_in_env Empty (TPoly k0 s) Star a p_emp_ks as Hfr;
       destruct Hfv; destruct Hfr;
-      try apply WFEEmpty; trivial.
+      try apply WFEEmpty; auto.
   - (* TLet e_x e *) apply thm_progress in p_e_t as Hprog; destruct Hprog.
     * (* e_x is a value *)
       apply lem_sem_det with (Let e_x e) e'' (subBV e_x e) in st_e_e'';
       try apply ELetV; try apply H2; subst e'';
       pose proof (fresh_not_elem nms) as Hy; set (y := fresh nms) in Hy;
       rewrite lem_subFV_unbind with y e_x e;
-      pose proof lem_subFV_notin as Hnot; destruct Hnot as [_ Hnot];
-      destruct Hnot as [Hnot _]; try rewrite <- Hnot with t y e_x;
+      pose proof lem_subFV_notin as Hnot; destruct Hnot as [_ [Hnot _]];
+      try rewrite <- Hnot with t y e_x;
       try apply lem_subst_typ_top with t_x;
       try rewrite <- lem_unbindT_lct with y t;
       try apply H0; try rewrite lem_unbindT_lct;
@@ -303,7 +294,7 @@ Proof. intros g e t e' p_e_t; revert e'; induction p_e_t;
       pose proof lem_fv_bound_in_fenv FEmpty (Let e_x e) 
                     (erase t) y p_exe_ert as Hfv;  
       pose proof lem_free_bound_in_env Empty t k y H as Hfr;
-      destruct Hfv; destruct Hfr; trivial;
+      destruct Hfv; destruct Hfr; auto;
       try apply not_elem_union_elim in H3; try destruct H3;
       try apply WFEEmpty; simpl; intuition.
     * (* e_x not value: *)
@@ -346,6 +337,218 @@ Proof. intros g e t e' p_e_t; revert e'; induction p_e_t;
     * (* otherw *) destruct H4 as [e0' st_e1_e1']; assert (e'' = If e0' e1 e2)
         by (apply lem_sem_det with (If e0 e1 e2); try apply EIf; assumption);
       subst e''; apply TIf with ps k nms; try assumption; apply IHp_e_t; trivial.
+  - (* TCons *) apply thm_progress in p_e_t1 as Hprog;
+    apply thm_progress in p_e_t2 as Hprog';
+    destruct Hprog; destruct Hprog';
+    (* eH not value: *)
+    try destruct H1 as [eH1 st_eH_eH1];
+    try apply lem_sem_det with (Cons eH eT) e'' (Cons eH1 eT) 
+      in st_e_e'' as He'';
+    try apply ECons1; try assumption; try subst e'';
+    try apply TCons; try apply IHp_e_t1; try apply p_e_t2; trivial; 
+    (* e' not a value *)
+    try destruct H2 as [eT1 st_eT_eT1];
+    try apply lem_sem_det with (Cons eH eT) e'' (Cons eH eT1) 
+      in st_e_e'' as He'';
+    try apply ECons2; try assumption; try subst e'';
+    try apply TCons; try apply p_e_t1; try apply IHp_e_t2; trivial.
+    (* both values *)
+    apply lem_value_stuck in st_e_e''; try apply val_Cons;
+    try assumption. contradiction.  
+  - (* TSwitch *) apply thm_progress in p_e_t as Hprog; 
+    destruct Hprog;
+    (* e not value: *)
+    try destruct H6 as [e' st_e_e'];
+    try apply lem_sem_det with (Switch e eN eC) e'' (Switch e' eN eC)
+      in st_e_e'' as He'';
+    try apply ESwitch; try assumption; try subst e'';
+    try apply TSwit with t ps k nms; try apply IHp_e_t; trivial.
+    (* e is a value *) 
+    apply lem_typing_hasftype in p_e_t as p_e_ert;
+    try apply lem_typing_wf in p_e_t as p_emp_t;
+    try simpl in p_e_ert; try apply WFEEmpty;
+    try apply lem_wftype_islct in p_emp_t as Hlct; 
+    unfold isLCT in Hlct; simpl in Hlct;
+    destruct Hlct as [Hlct Hlcp1];
+    pose proof lem_open_at_lc_at as [Hope [Hopt _]];
+    apply lemma_list_values in p_e_ert as Hfval; 
+    try apply H6; destruct e eqn:E; simpl in Hfval; try contradiction.
+    * (* e = Nil *) clear H3 H5 IHp_e_t.
+      apply lem_sem_det with (Switch Nil eN eC) e'' eN 
+        in st_e_e'' as He''; try apply ESwitchN; subst e''.
+      
+      try apply lem_invert_nil in p_e_t as Hinv ; 
+      try destruct Hinv 
+        as [s' [p_s'_t [p_emp_s' [Hs'1 [Hs'2 p_ls'_ltps]]]]];
+      try inversion p_ls'_ltps;
+      try apply lem_wftype_islct in p_emp_s' as Hlcs';
+      try unfold isLCT in Hlcs';
+      try apply WFEEmpty; try apply p_emp_t.
+      
+      pose proof (fresh_varE_not_elem (union nms nms0) Empty (Annot eN t')) 
+        as Hy; 
+      set (y := fresh_varE (union nms nms0) Empty (Annot eN t')) in Hy. 
+      simpl in Hy; destruct Hy as [Hfv [Hftv [Hnms Hemp]]]. 
+      apply not_elem_union_elim in Hnms; destruct Hnms;
+      apply not_elem_union_elim in Hfv; destruct Hfv as [Hfv Hfv'];
+      apply not_elem_union_elim in Hftv; destruct Hftv as [Hftv Hftv'];
+      pose proof lem_subFV_notin as Hnot. 
+      destruct Hnot as [Hnot_e [Hnot_t _]].
+
+      rewrite <- Hnot_e with eN y Nil; 
+      try rewrite <- Hnot_t with t' y Nil;
+      try apply lem_subst_typ_top 
+        with (TList t (PCons (eq (Ic 0) (length t (BV 0))) ps));
+      try apply H2; 
+      try apply TSub 
+        with (TList s' (PCons (eq (Ic 0) (length s' (BV 0))) PEmpty)) Star;
+      try apply TNil with Star;
+      try apply lem_wflist_len_zero;
+
+      try apply SList with (union nms nms0);
+      try apply p_s'_t; intros;
+      try apply not_elem_union_elim in H14; try destruct H14;
+      try apply WFEEmpty; auto.
+
+      assert (
+        unbindP y0 (PCons (eq (Ic 0) (length t (BV 0))) ps)
+            = strengthen 
+                (unbindP y0 (PCons (eq (Ic 0) (length t (BV 0))) PEmpty)) 
+                (unbindP y0 ps) )
+        as Hpred by reflexivity; try rewrite Hpred.
+      apply IConj; try apply H11;
+      unfold unbindP; simpl;
+      try rewrite Hopt with t  0 0 y0;
+      try rewrite Hopt with s' 0 0 y0;
+      try apply ILenSub; 
+      try apply lem_weaken_subtype_top with Star Star;
+      try apply (lem_wflist_wftype Empty t ps Star);
+      try apply WFEEmpty; trivial. 
+    * (* e = Cons v1 v2 *)  clear H3 H5 IHp_e_t.
+      inversion H6; subst e0_1 e0_2.
+      apply lem_sem_det 
+        with (Switch (Cons v1 v2) eN eC) e'' (App (App eC v1) v2) 
+        in st_e_e'' as He''; try apply ESwitchC;
+        try assumption; subst e''. 
+
+      pose proof (fresh_varE_not_elem nms Empty eC) as Hy; 
+      set (y := fresh_varE nms Empty eC) in Hy. 
+      simpl in Hy; destruct Hy as [Hfv [Hftv [Hnms Hemp]]].   
+      apply lem_free_bound_in_env with Empty t' k y in H1 as Hfr'; 
+      try apply Hemp; destruct Hfr' as [Hfr' _].
+      apply lem_free_bound_in_env with Empty (TList t ps) Star y 
+        in p_emp_t as Hfr;  
+      try apply Hemp; destruct Hfr as [Hfr _]; simpl in Hfr;
+      apply not_elem_union_elim in Hfr; destruct Hfr as [Hfr HfvP].
+      pose proof lem_subFV_notin as Hnot; 
+      destruct Hnot as [Hnot_e [Hnot_t _]].
+
+      apply TSub with 
+        (TExists (TList t (PCons (eq (length t (Cons v1 v2)) 
+                                     (App (Prim Succ) (length t (BV 0))))
+                                 PEmpty))
+                 t') Star;
+      try apply TApp;
+      try match goal with
+          | [ |- Hastype _ (App eC v1) ?ltt' ]
+                => apply TSub with (TExists t ltt') Star
+          end;
+        (*  (TFunc (TList t (PCons (eq (length t (Cons v1 v2)) 
+                                     (App (Prim Succ) (length t (BV 0))))
+                                 PEmpty))
+                 t')) Star.*)
+      try apply TApp;      
+      (* eC typing: substitution *)
+      try rewrite <- Hnot_e with eC y (Cons v1 v2);
+      try assert (y =? y = true) by (apply Nat.eqb_eq; reflexivity);
+      try assert (
+        TFunc t (TFunc (TList t (PCons (eq (length t (Cons v1 v2)) 
+                                           (App (Prim Succ) (length t (BV 0)))) 
+                                PEmpty)) t')
+          = tsubFV y (Cons v1 v2)
+              (TFunc t (TFunc (TList t (PCons (eq (length t (FV y))
+                                                  (App (Prim Succ) (length t (BV 0)))) 
+                                      PEmpty)) t'))
+      ) as Htsub by (unfold eq; unfold length; unfold tsubFV; 
+                     fold tsubFV; fold subFV; rewrite Hnot_t; 
+                     try rewrite H3; try rewrite Hnot_t; trivial);
+      try rewrite Htsub;
+      try apply lem_subst_typ_top with (TList t ps);
+      try apply H4; 
+      try apply wfenv_unique; try apply WFEEmpty; trivial;
+      (* v1 typing: inversion lemma *)
+      apply lem_invert_tlist in p_e_t as Hv1v2;
+      try apply WFEEmpty; trivial;
+      destruct Hv1v2 as [qs [p_v1_t p_v2_tqs]];
+      try apply p_v1_t.
+      (* v2 typing: inversion lemma *)
+      Focus 3. pose proof TCons.
+
+      (* 2x subtyping: SBind *)
+      (* 2x wellformedness *)
+      
+      try apply H4. apply H4.
+      
+      
+      apply not_elem_union_elim in Hfv; apply not_elem_union_elim in Hftv; 
+
+      rewrite <- Hnot_e with eN y Nil; 
+      try rewrite <- Hnot_t with t' y Nil;
+      try apply lem_subst_typ_top 
+        with (TList t (PCons (eq (Ic 0) (length t (BV 0))) ps));
+
+      try apply TSub 
+        with (TList t (PCons (eq (Ic 0) (length t (BV 0))) PEmpty)) Star;
+        
+        try apply TNil with Star; intuition.
+      
+      Focus 3.
+      apply SList with nms; intros.
+      Focus 2.
+      pose IStren.
+      assert ( unbindP y0 (PCons (eq (Ic 0) (length t (BV 0))) PEmpty)
+        = strengthen (PCons (eq (Ic 0) (length t (FV y0))) PEmpty) 
+                     (unbindP y0 PEmpty) )
+
+        as Hprd1 by (
+        unfold unbindP; unfold eq; unfold length; simpl; 
+                      rewrite Hopt with t 0 0 y0; trivial);
+      rewrite Hprd1.
+      assert ( unbindP y0 (PCons (eq (Ic 0) (length t (BV 0))) ps)
+        = strengthen (PCons (eq (Ic 0) (length t (FV y0))) PEmpty) 
+                     (unbindP y0 ps) )
+
+        as Hprd2 by (
+        unfold unbindP; unfold eq; unfold length; simpl; 
+                      rewrite Hopt with t 0 0 y0; trivial);
+      rewrite Hprd2.
+      apply IStren.
+
+      Lemma lem_narrow_typ_top : 
+  forall (g:env) (x:vname) (s_x t_x:type) (k_sx k_tx:kind) (e:expr) (t:type),
+    Hastype (ECons x t_x g) e t
+            -> unique g -> ~ (in_env x g) 
+            -> WFtype g s_x k_sx -> WFtype g t_x k_tx -> Subtype g s_x t_x -> WFEnv g
+            -> Hastype (ECons x s_x g) e t .
+
+      try apply TSub 
+        with (TList t (PCons (eq (Ic 0) (length t (BV 0))) ps)) Star;
+      try apply WFEEmpty; intuition.
+      apply TNil with Star.
+
+      pose proof TNil.
+      
+      apply H2 with y.
+
+      try apply H0; try apply H2; try apply lem_exact_type;
+      trivial; try apply WFEEmpty;
+      inversion p_emp_t; apply H6.
+
+    * (* e = Cons v1 v2 *)
+      apply lem_sem_det 
+        with (Switch (Cons v1 v2) eN eC) e'' (App (App eC v1) v2)
+        in st_e_e'' as He''; try apply ESwitchC; subst e''.
+
   - (* TSub e, s <: t *) apply TSub with s k; try apply IHp_e_t; trivial.
   Qed.
   
